Proved fold' and max_set_of_list_subset_exists

src/Union.lean
@@ -1,12 +1,23 @@
 import data.finset
 import data.set.lattice
 import util
+import seq
 
 universes u v w x
 variables {α : Type u} {β : Type v} {γ : Type w} {ι : Type x}
 
 def fold' : Π {α : Type u} (C : list α → Sort v) (l : list α), 
-    C [] → (Π (e : α) (l' : list α), e ∈ l → l' ⊆ l → C l' → C (e :: l')) → C l := sorry
+    C [] → (Π (e : α) (l' : list α), e ∈ l → l' ⊆ l → C l' → C (e :: l')) → C l
+| α C [] := λ h_nil ih, by assumption
+| α C [hd] := λ h_nil ih, by apply ih hd [] (list.mem_singleton_self hd) (list.nil_subset [hd]) h_nil
+| α C (hd :: tl_hd :: tl_tl) := λ h_nil ih, 
+begin
+    apply ih hd (tl_hd :: tl_tl) (list.mem_cons_self hd (tl_hd :: tl_tl)) (list.subset_cons hd (tl_hd :: tl_tl)),
+    have ih' : Π (e : α) (l' : list α), e ∈ (list.cons tl_hd tl_tl) → l' ⊆ (tl_hd :: tl_tl) → C l' → C (e :: l'),
+    intros e l' e_mem l'_sub,
+    apply ih e l' ((list.mem_cons_iff e hd (tl_hd :: tl_tl)).2 (or.inr e_mem)) (list.subset_cons_of_subset hd l'_sub),
+    apply fold' C (tl_hd :: tl_tl) h_nil ih',
+end
 
 def flatten : ∀ (l : list α), (α → set β) → set β
 | [] := λ f, ∅ 
@@ -16,57 +27,48 @@ def flatten : ∀ (l : list α), (α → set β) → set β
 @[simp] lemma flatten_cons : ∀ {f : α → set β} {hd : α} {tl : list α}, flatten (hd :: tl) f = f hd ∪ flatten tl f := λ f hd tl, rfl
 
 namespace set
-variables [comm_ring β] [decidable_eq β] [lattice.semilattice_sup_bot ι] [decidable_rel ((≤) : ι → ι → Prop)] [is_total ι (≤)] [decidable_eq ι]
+variables [decidable_eq β]
 
-instance : decidable_linear_order ι := 
-    { decidable_le := _inst_4,
-      decidable_eq := _inst_6,
-      le_total := is_total.total (≤),
-    .. _inst_3 }
-
-lemma union_of_head_le {s : ι → set β} {hd tl_hd : ι} {tl_tl : list ι} (h : hd ≤ tl_hd) :
-     s tl_hd ∪ s (list.foldl max hd tl_tl) = s tl_hd ∪ s (list.foldl max tl_hd tl_tl) :=
+lemma flatten_eq_max (s : seqR.seq_R (set β) (<)) (hd : ℕ) (tl : list ℕ) : flatten (hd :: tl) s.1 = s.1 (tl.foldr max hd) :=
 begin
-    revert hd tl_hd, induction tl_tl; intros,
-    simp,
-end
-
-lemma flatten_eq_max {s : ι → set β} {hd : ι} {tl : list ι} : flatten (hd :: tl) s = s (tl.foldl max hd) :=
-begin
-    induction tl; simp at *,
-    from if h : hd ≤ tl_hd
+    induction tl; simp at *, 
+    rw [←union_assoc, union_comm (s.1 hd), union_assoc, tl_ih],
+    from if h : tl_hd ≥ (list.foldr max hd tl_tl)
     then begin
-        rw [max_eq_right h, ←union_assoc, union_comm (s hd), union_assoc, tl_ih],
+        rw max_eq_left h,
+        have H : s.val (list.foldr max hd tl_tl) ⊆ s.val tl_hd, apply seqR.le_trans_of_lt s h,
+        rw union_eq_self_of_subset_right H,
     end
-    else sorry
+    else begin
+        rw max_eq_right (le_of_not_ge h),
+        have H : s.val tl_hd ⊆ s.val (list.foldr max hd tl_tl), apply seqR.le_trans_of_lt s (le_of_not_ge h),
+        rw union_eq_self_of_subset_left H,
+    end
 end
 
-
-set_option trace.simplify.rewrite true
-def mem_set_max {s : ι → set β} {gs : list β} (h : ↑(gs.to_finset) ⊆ Union s) : 
-    ∃ i : ι, ↑(gs.to_finset) ⊆ s i ∧ s i ⊆ Union s := 
+lemma max_set_of_list_subset_exists {s : seqR.seq_R (set β) (<)} {gs : list β} (h : ↑(gs.to_finset) ⊆ Union (λ (i : ℕ), (s.1 i))) : 
+    ∃ i : ℕ, ↑(gs.to_finset) ⊆ s.1 i ∧ s.1 i ⊆ Union (λ (i : ℕ), (s.1 i)) :=
 begin
-    --simp [has_subset.subset, set.subset] at h,
-    have H := fold' (λ l : list β, (∃ i : list ι, ↑l.to_finset ⊆ flatten i s)) gs (by simp) 
-        (begin 
-            intros, rw list.mem_to_set at a,
-            have h' := h a, simp at h',
-            cases h', cases a_2,
-            apply exists.intro (list.cons h'_w a_2_w), 
-            change (list.to_finset (e :: l')).to_set ⊆ s h'_w ∪ flatten a_2_w s,
+    have H := fold' (λ l : list β, (∃ i : list ℕ, ↑l.to_finset ⊆ flatten i s.1)) gs (by simp)
+        (begin
+            intros e l' e_mem l'_sub ih, rw list.mem_to_set at e_mem,
+            have e_mem' := h e_mem, simp at e_mem',
+            cases e_mem', cases ih,
+            apply exists.intro (list.cons e_mem'_w ih_w),
+            change (list.to_finset (e :: l')).to_set ⊆ s.1 e_mem'_w ∪ flatten ih_w s.1,
             intros x hx, rw ←list.mem_to_set at hx,
             simp,
-            cases hx, rw hx at *, apply or.inl h'_h,
+            cases hx, rw hx at *, apply or.inl e_mem'_h,
             have hx' : x ∈ l'.to_finset.to_set,
                 rw ←list.mem_to_set, unfold has_mem.mem, assumption,
-            apply or.inr (a_2_h hx'),
+            apply or.inr (ih_h hx'),
         end),
     cases H,
-    cases H_w, simp [subset_empty_iff] at H_h, rw H_h, apply exists.intro (⊥ : ι),
-    apply and.intro; simp [Union, lattice.supr, lattice.Sup, range, lattice.has_Sup.Sup, lattice.complete_lattice.Sup],
-    intros a ha, simp, apply exists.intro (s ⊥), finish,
-    have H_h' : flatten (list.cons H_w_hd H_w_tl) s = s ((list.cons H_w_hd H_w_tl).foldl max H_w_hd),
-    induction H_w_tl; simp,
+    cases H_w, simp [subset_empty_iff] at H_h, rw H_h, apply exists.intro 0,
+    apply and.intro, simp, apply subset_Union,
+    rw flatten_eq_max s H_w_hd H_w_tl at H_h,
+    apply exists.intro (list.foldr max H_w_hd H_w_tl), 
+    apply and.intro H_h, apply subset_Union,
 end
 
 end set
