src/seq.lean
@@ -44,6 +44,29 @@ def nth (s: seq_R α R) (n: ℕ): α := s.1 n
 
 def no_inf_chain (α: Type*) (R: α → α → Prop): Prop := ¬' seq_R α R
 
+
+section preorder
+variables [partial_order α]
+
+protected lemma lt_trans_of_lt (s : seq_R α (<)) : ∀ {m n}, m < n → (s.1 m) < (s.1 n) :=
+λ m n hmn, begin
+    rw ←nat.add_sub_cancel' hmn,
+    apply @nat.strong_induction_on (λ x, (s.val m) < (s.val ((m + 1) + x))) (n - (m + 1)),
+    intros k ih,
+    cases k, apply s.2,
+    have h := ih k (nat.lt_succ_self k),
+    apply lt_trans h (s.2 (m + 1 + k)),
+end
+
+protected lemma le_trans_of_lt (s : seq_R α (<)) : ∀ {m n}, m ≤ n → s.1 m ≤ s.1 n :=
+λ m n hmn, begin
+    from if h : m = n
+    then by finish
+    else by apply le_of_lt (lt_trans s (lt_of_le_of_ne hmn h))
+end
+
+end preorder
+
 end seq
 
 variable (α : Type u)
